---
title: "Assignment 4"
author: "Thrisha Rajkumar"
date: "`r Sys.Date()`"
output:
  pdf_document:
    latex_engine: xelatex
---



## Q1.
The following function performs imputation by mean. What library do we need 
to load to run this function? 

```{r}
# Adding tidyverse to run this function 
library(tidyverse) 
```

```{r}

impute_by_mean<-function(x){ 
mu<-mean(x,na.rm=TRUE) # first compute the mean of x 
  impute_f<-function(z){ # coordinate-wise imputation 
    if(is.na(z)){ 
      return(mu) # if z is na replace with mean 
      }else{ 
        return(z) # otherwise leave in place 
      } 
    } 
return(map_dbl(x,impute_f)) # apply the map function to impute across 
vector 
}
```

## Q2. 
Create a function called â€œimpute_by_medianâ€ which imputes missing values 
based on the median of the sample, rather than the mean. 

```{r}
impute_by_median <- function(x) {
  median_of_x <- median(x, na.rm = TRUE)  # first compute the median of x
  
  replace_function <- function(y) {
    if (is.na(y)) {  # correct reference to 'y' instead of 'z'
      return(median_of_x)
    } else {
      return(y)
    }
  }
  return(map_dbl(x, replace_function))  # Apply function to impute missing values
}

v <- c(1, 2, NA, 4)
impute_by_median(v)

impute_by_median(v) 

```

## Q2. 
## Question
Generate a data frame `df_xy` with the following specifications:

1. The variable `x` is a sequence defined as:
   - Starting value: 0
   - Ending value: 10
   - Increment: 0.1

2. The variable `y` is calculated as `y = 5x + 1` for each corresponding value of `x`.

3. Place these variables into a data frame called `df_xy`.

4. Display the first few rows of the data frame.

```{r}
x <- seq(from = 0, to=10, by=0.1)
y <- x*5 + 1
df_xy = data.frame(x,y)
df_xy %>% head(5)
```

## Q3.
map2: 
The â€œmap2()â€ function is similar to the â€œmap()â€ function but iterates over two 
variables in parallel rather than one. You can learn more here 
https://purrr.tidyverse.org/reference/map2.html. The following simple example 
shows you how â€œmap2_dbl()â€ can be combined with the â€œmutate()â€ function. 

```{r}
df_xy %>% 
  mutate(z=map2_dbl(x,y,~.x+.y)) %>% 
  head(5) 
```

use map2_dbl() to generate a new data frame with missing data. 
First create a function â€œsometimes_missingâ€ with two arguments: â€œindexâ€ and 
â€œvalueâ€. The â€œfunctionâ€ should return â€œNAâ€ if index is divisible by 5 and returns value 
otherwise. 
```{r}
sometimes_missing <- function(index, value){
  if(index%%5==0){
    return(NA)
  }else{
    return(value)
  }
}
sometimes_missing(14,25) 
```

we need to generate "df_xy_missing" with two variables x and y

"d_xy_missing" 
"row_number(),
map2_dbl(), 
mutate() 

```{r}
df_xy_missing <- df_xy %>% 
  mutate(y=map2_dbl(row_number(),y,sometimes_missing)) 
df_xy_missing<-df_xy  %>% 
  mutate(y=map2_dbl(.x=row_number(),.y=y,sometimes_missing)) 
df_xy_missing %>% head(10) 
```

## Q5.
(Q5) Create a new data frame â€œdf_xy_imputedâ€ with two variables ğ‘¥ and ğ‘¦. For the 
first variable ğ‘¥ we have a sequence (ğ‘¥ ,â‹¯,ğ‘¥ ), which is precisely the same as with 
â€œdf_xyâ€. For the second variable ğ‘¦ we have a sequence (ğ‘¦â€² ,â‹¯,ğ‘¦â€² ) which is formed 
from (ğ‘¦ ,â‹¯,ğ‘¦) by imputing any missing values with the median. To generate 
â€œdf_xy_imputedâ€ from â€œdf_xy_missingâ€ by applying a combination of the functions 
â€œmutate()â€ and â€œimpute_by_median()â€. 

```{r}
df_xy_impute<-df_xy_missing %>%  
mutate(y=impute_by_median(y)) 
head(df_xy_impute)
```


## Tidying data with pivot functions
â€œâ€œHockeyLeague.csvâ€â€œ downloaded

```{r}

library(readxl) # load the readxl library 
folder_path <- "C:/Users/pc/Desktop/R-Programming - SCEM/Assignment 4"
file_name <- "HockeyLeague.xlsx"
file_path <- paste0(folder_path, "/", file_name)

wins_data_frame <- read_excel(file_path, sheet="Wins") # read a sheet from an xl file 

wins_data_frame %>% 
  select(1:5) %>% 
  head(3)

```

### (Q1) 

```{r}
w_l_narrow<-function(w_or_l){ 
return( 
read_excel(file_path,sheet=w_or_l)%>% 
rename(Team=...1)%>% 
pivot_longer(!Team,names_to="Year",values_to="val")%>% 
mutate(Year=as.integer(Year))%>% 
separate(col=val,into=c(w_or_l,"Total"),sep=" of ",convert=TRUE) ) 
} 
wins_tidy<-w_l_narrow(w_or_l="Wins") 
wins_tidy %>% dim()
wins_tidy%>%head(5) 
```

#### (Q2)

```{r}
losses_tidy<-w_l_narrow(w_or_l="Losses") 
losses_tidy %>% head(5) 
```

### (Q3)

```{r}
hockey_df<-inner_join(wins_tidy,losses_tidy)%>% 
  mutate(Draws=Total-Wins-Losses)%>% 
  mutate(across(starts_with(c("Wins","Losses","Draws")),~.x/Total, .names="{.col}_rt")) 
hockey_df %>% head(5)
```

### (Q4) 

```{r}
hockey_df %>%  
  select(-Wins,-Draws,-Losses) %>% 
  group_by(Team) %>% 
  summarise(across(starts_with(c("Wins","Losses","Draws")), 
                   list(md=median,mn=mean), 
                   .names="{substring(.col,1,1)}_{.fn}")) %>% 
  arrange(desc(W_md)) 
```

## 1.3 Simulation experiments of probabilities

```{r}
num_red_balls<-3 
num_blue_balls<-7 
total_draws<-22 
prob_red_spheres<-function(z){ 
  total_balls<-num_red_balls+num_blue_balls 
  log_prob<-log(choose(total_draws,z))+ 
    z*log(num_red_balls/total_balls)+(total_draws-z)*log(num_blue_balls/total_balls) 
  return(exp(log_prob)) 
} 
 
itermap <- function(.x, .f) { 
  result <- list() 
  for (item in .x) { result <- c(result, list(.f(item))) } 
  return(result) 
} 
 
itermap_dbl <- function(.x, .f) { 
  result <- numeric(length(.x)) 
  for (i in 1:length(.x)) { result[i] <- .f(.x[[i]]) } 
  return(result) 
} 
 
num_trials<-1000 # set the number of trials 
set.seed(0) # set the random seed 
 
num_reds_in_simulation <- data.frame(trial=1:num_trials) %>% 
  mutate(sample_balls = itermap(.x=trial, function(x){sample(10,22, replace = TRUE)})) %>%  
  mutate(num_reds = itermap_dbl( .x=sample_balls, function(.x) sum(.x<=3) ) ) %>%  
  pull(num_reds)  
 
prob_by_num_reds <- data.frame(num_reds=seq(22)) %>%  
  mutate(TheoreticalProbability=prob_red_spheres(num_reds)) %>%  
  mutate(EstimatedProbability= 
           itermap_dbl(.x=num_reds, function(.x) sum(num_reds_in_simulation==.x))/num_trials) 
num_red_balls<-3 
num_blue_balls<-7 
total_draws<-22 
prob_red_spheres<-function(z){ 
  total_balls<-num_red_balls+num_blue_balls 
  log_prob<-log(choose(total_draws,z))+ 
    z*log(num_red_balls/total_balls)+(total_draws-z)*log(num_blue_balls/total_balls) 
  return(exp(log_prob)) 
} 
 
num_trials<-1000 # set the number of trials 
set.seed(0) # set the random seed 
 
num_reds_in_simulation <- data.frame(trial=1:num_trials) %>% 
  mutate(sample_balls = map(.x=trial, ~sample(10,22, replace = TRUE))) %>%  
  mutate(num_reds = map_dbl( .x=sample_balls, ~sum(.x<=3) ) ) %>%  
  pull(num_reds)  
 
prob_by_num_reds <- data.frame(num_reds=seq(22)) %>%  
  mutate(TheoreticalProbability=prob_red_spheres(num_reds)) %>%  
  mutate(EstimatedProbability=map_dbl(.x=num_reds, ~sum(num_reds_in_simulation==.x))/num_trials) 
```

## Q2

```{r}
prob_by_num_reds %>% 
  pivot_longer(cols=c("EstimatedProbability","TheoreticalProbability"),
  
               names_to="Type",values_to="count") %>% 
  ggplot(aes(num_reds,count)) +  
  geom_line(aes(linetype=Type, color=Type)) + geom_point(aes(color=Type
 )) + 
  scale_linetype_manual(values = c("solid", "dashed"))+ 
  theme_bw() + xlab("Number of reds") + ylab("Probabilities") 

```


### 2. Conditional probability, Bayes rule and independence


### Bayes' Theorem

Given events \( A, B \in \mathcal{E} \) with \( \mathbb{P}(A) > 0 \) and \( \mathbb{P}(B) > 0 \), we have:

\[
\mathbb{P}(B \mid A) = \frac{\mathbb{P}(B) \cdot \mathbb{P}(A \mid B)}{\mathbb{P}(A)}
\]

### The Law of Total Probability

the law of total probability:

\[
\mathbb{P}(B) = \sum_i \mathbb{P}(A_i \cap B) = \sum_i \mathbb{P}(B \mid A_i) \cdot \mathbb{P}(A_i)
\]

### Independent and Dependent Events

Let \( (\Omega, \mathcal{E}, \mathbb{P}) \) be a probability space. We define the following:

1. A pair of events \( A, B \in \mathcal{E} \) are said to be independent if:

\[
\mathbb{P}(A \cap B) = \mathbb{P}(A) \cdot \mathbb{P}(B)
\]

2. A pair of events \( A, B \in \mathcal{E} \) are said to be dependent if:

\[
\mathbb{P}(A \cap B) \neq \mathbb{P}(A) \cdot \mathbb{P}(B)
\]

## 2.1  Bayes theorem 
### (Q1) 

```{r}
p_A<-0.9 
p_B_given_A<-0.8 
p_not_B_given_not_A<-0.75 
p_B<-p_B_given_A*p_A+(1-p_not_B_given_not_A)*(1-p_A) 
p_A_given_B<-p_B_given_A*p_A/p_B 
p_A_given_B 
```

## 2.2 Conditional probabilities 
### (Q1) 

## Conditional Probabilities

### (Q1) Suppose we have a probability space \( (\Omega, \mathcal{E}, \mathbb{P}) \).

#### (a) Expression for \( \mathbb{P}(A \mid B) \) when \( A \subseteq B \) and \( \mathbb{P}(B) \neq 0 \)
We are given \( A \subseteq B \), which implies that \( A \cap B = A \). By the definition of conditional probability, we have:

\[
\mathbb{P}(A \mid B) = \frac{\mathbb{P}(A \cap B)}{\mathbb{P}(B)} = \frac{\mathbb{P}(A)}{\mathbb{P}(B)}
\]

Thus, the conditional probability of \( A \) given \( B \) is:

\[
\mathbb{P}(A \mid B) = \frac{\mathbb{P}(A)}{\mathbb{P}(B)}
\]

#### (b) If additionally, \( \mathbb{P}(B \setminus A) = 0 \), what is \( \mathbb{P}(A \mid B) \)?
If \( \mathbb{P}(B \setminus A) = 0 \), then \( B \subseteq A \), which means that \( A = B \). Therefore, we have:

\[
\mathbb{P}(A \mid B) = \frac{\mathbb{P}(A)}{\mathbb{P}(B)} = 1
\]

Thus, \( \mathbb{P}(A \mid B) = 1 \) when \( B \subseteq A \) and \( \mathbb{P}(B \setminus A) = 0 \).

#### (c) Suppose \( A \cap B = \emptyset \). What is \( \mathbb{P}(A \mid B) \)?
If \( A \cap B = \emptyset \), then \( \mathbb{P}(A \cap B) = 0 \). The conditional probability \( \mathbb{P}(A \mid B) \) is given by:

\[
\mathbb{P}(A \mid B) = \frac{\mathbb{P}(A \cap B)}{\mathbb{P}(B)} = \frac{0}{\mathbb{P}(B)} = 0
\]

Thus, \( \mathbb{P}(A \mid B) = 0 \) when \( A \cap B = \emptyset \).

#### (d) Does the result still hold for \( \mathbb{P}(A \cap B) = 0 \)?
If \( \mathbb{P}(A \cap B) = 0 \), then the result still holds: 

\[
\mathbb{P}(A \mid B) = 0
\]

This is because if \( A \cap B = \emptyset \), then \( \mathbb{P}(A \mid B) = 0 \), and if \( \mathbb{P}(A \cap B) = 0 \), the numerator of the conditional probability is zero, leading to the same conclusion.

#### (e) Suppose \( B \subseteq A \). What is \( \mathbb{P}(A \mid B) \)?
If \( B \subseteq A \), then \( A \cap B = B \), and the conditional probability is:

\[
\mathbb{P}(A \mid B) = \frac{\mathbb{P}(A \cap B)}{\mathbb{P}(B)} = \frac{\mathbb{P}(B)}{\mathbb{P}(B)} = 1
\]

Thus, \( \mathbb{P}(A \mid B) = 1 \) when \( B \subseteq A \).

#### (f) Is \( \mathbb{P}(A \mid \Omega) \) equal to \( \mathbb{P}(A) \)? Why?
Yes, \( \mathbb{P}(A \mid \Omega) \) is equal to \( \mathbb{P}(A) \). This is because the probability of \( A \) conditioned on the entire sample space \( \Omega \) is simply the probability of \( A \):

\[
\mathbb{P}(A \mid \Omega) = \frac{\mathbb{P}(A \cap \Omega)}{\mathbb{P}(\Omega)} = \frac{\mathbb{P}(A)}{1} = \mathbb{P}(A)
\]

Thus, \( \mathbb{P}(A \mid \Omega) = \mathbb{P}(A) \).

#### (g) Show that \( \mathbb{P}(A \cap B \cap C) = \mathbb{P}(A \mid B \cap C) \cdot \mathbb{P}(B \mid C) \cdot \mathbb{P}(C) \)
We want to express \( \mathbb{P}(A \cap B \cap C) \) in terms of conditional probabilities. First, let \( D = B \cap C \). Then, by the chain rule of probability:

\[
\mathbb{P}(A \cap B \cap C) = \mathbb{P}(A \cap D) = \mathbb{P}(A \mid D) \cdot \mathbb{P}(D)
\]

Now, \( \mathbb{P}(D) = \mathbb{P}(B \cap C) = \mathbb{P}(B \mid C) \cdot \mathbb{P}(C) \). Substituting this into the equation:

\[
\mathbb{P}(A \cap B \cap C) = \mathbb{P}(A \mid B \cap C) \cdot \mathbb{P}(B \mid C) \cdot \mathbb{P}(C)
\]

#### (h) Show that \( \mathbb{P}(A \cap B \cap C) = \mathbb{P}(B \mid A \cap C) \cdot \mathbb{P}(A \mid C) \cdot \mathbb{P}(C) \)
We proceed similarly. Again, let \( D = A \cap C \). Then:

\[
\mathbb{P}(A \cap B \cap C) = \mathbb{P}(B \cap D) = \mathbb{P}(B \mid D) \cdot \mathbb{P}(D)
\]

Now, \( \mathbb{P}(D) = \mathbb{P}(A \cap C) = \mathbb{P}(A \mid C) \cdot \mathbb{P}(C) \). Substituting this:

\[
\mathbb{P}(A \cap B \cap C) = \mathbb{P}(B \mid A \cap C) \cdot \mathbb{P}(A \mid C) \cdot \mathbb{P}(C)
\]

#### (i) Show that if \( \mathbb{P}(B \cap C) \neq 0 \), we have:

\[
\mathbb{P}(A \mid B \cap C) = \frac{\mathbb{P}(A \cap B \cap C)}{\mathbb{P}(B \cap C)} = \mathbb{P}(A \mid B \cap C)
\]

This result is consistent with the previous findings, as it shows the relationship between conditional probabilities when the intersection of \( B \) and \( C \) is nonzero.

### (Q2) 

## Conditional Probability Example

Let \( A \) be the event that the flight is **not cancelled**, and \( B \) be the event that it is **windy**. 

We are given the following conditional probabilities:

\[
\mathbb{P}(A \mid B) = 1 - 0.3 = 0.7
\]
and 
\[
\mathbb{P}(A \mid B^c) = 1 - 0.1 = 0.9
\]
where \( B^c \) is the complement of \( B \) (i.e., the event that it is **not windy**).

By the **law of total probability**, we can express \( \mathbb{P}(A) \) as:

\[
\mathbb{P}(A) = \mathbb{P}(A \mid B) \mathbb{P}(B) + \mathbb{P}(A \mid B^c) \mathbb{P}(B^c)
\]

Substituting the given values:

\[
\mathbb{P}(A) = (0.7 \cdot 0.8) + (0.9 \cdot 0.2) = 0.56 + 0.18 = 0.86
\]

Thus, the probability that the flight is not cancelled is \( \mathbb{P}(A) = 0.86 \).

### 2.3 Mutual independence and pair-wise independent 
### Q1

## Independence of Events Example

We are given the following probabilities:

\[
\mathbb{P}(\{(0,0,0)\}) = \mathbb{P}(\{(0,1,1)\}) = \mathbb{P}(\{(1,0,1)\}) = \mathbb{P}(\{(1,1,0)\}) = \frac{1}{4}
\]

From this, we can deduce:

\[
\mathbb{P}(A) = \mathbb{P}(B) = \mathbb{P}(C) = \frac{1}{2}
\]

### Pairwise Independence

Since each of the intersections \( A \cap B \), \( A \cap C \), and \( B \cap C \) has only one element, we have:

\[
\mathbb{P}(A \cap B) = \frac{1}{4} = \left(\frac{1}{2}\right) \cdot \left(\frac{1}{2}\right) = \mathbb{P}(A) \cdot \mathbb{P}(B)
\]

\[
\mathbb{P}(A \cap C) = \frac{1}{4} = \left(\frac{1}{2}\right) \cdot \left(\frac{1}{2}\right) = \mathbb{P}(A) \cdot \mathbb{P}(C)
\]

\[
\mathbb{P}(C \cap B) = \frac{1}{4} = \left(\frac{1}{2}\right) \cdot \left(\frac{1}{2}\right) = \mathbb{P}(C) \cdot \mathbb{P}(B)
\]

Thus, \( A \), \( B \), and \( C \) are **pairwise independent**.

### Mutual Independence

On the other hand, we have:

\[
A \cap B \cap C = \emptyset \quad \text{and} \quad \mathbb{P}(A \cap B \cap C) = 0
\]

Now, we check if the events are mutually independent. The product of the individual probabilities is:

\[
\mathbb{P}(A) \cdot \mathbb{P}(B) \cdot \mathbb{P}(C) = \frac{1}{2} \cdot \frac{1}{2} \cdot \frac{1}{2} = \frac{1}{8}
\]

Since:

\[
\mathbb{P}(A \cap B \cap C) = 0 \quad \text{and} \quad \mathbb{P}(A) \cdot \mathbb{P}(B) \cdot \mathbb{P}(C) = \frac{1}{8}
\]

we conclude that \( A \), \( B \), and \( C \) are **not mutually independent**.
